rocq/theories/TypeSystem/EnvRootSoundness.v
@@ -1629,43 +1629,30 @@ Proof.
       destruct (first_duplicate_branch l) as [dup |] eqn:Hdup; try discriminate.
       destruct (first_unknown_variant_branch l (enum_variants edef)) as [unknown |]
         eqn:Hunknown; try discriminate.
-      destruct (first_unsupported_match_payload l (enum_variants edef)) as [payload |]
-        eqn:Hunsupported; try discriminate.
-      destruct (first_unsupported_match_payload_none _ _ Hunsupported)
-        as [Hbinders Hpayload].
       destruct (first_missing_variant_branch (enum_variants edef) l) as [missing |]
         eqn:Hmissing; try discriminate.
       destruct (enum_variants edef) as [|v_head v_tail] eqn:Hvariants;
         try discriminate.
       simpl in Hinfer.
+      destruct (lookup_expr_branch_binders (enum_variant_name v_head) l)
+        as [binders_head |] eqn:Hbinders_head; try discriminate.
       destruct (lookup_branch_b (enum_variant_name v_head) l) as [e_head |]
-        eqn:Hlookup_branch.
-      2: {
-        destruct (lookup_expr_branch_binders (enum_variant_name v_head) l);
-          discriminate.
-      }
-      assert (Hfields_head : enum_variant_fields v_head = []).
-      {
-        simpl in Hpayload.
-        destruct (enum_variant_fields v_head) eqn:Hfields; [reflexivity | discriminate].
-      }
-      assert (Hbinders_head :
-        lookup_expr_branch_binders (enum_variant_name v_head) l = Some []).
-      {
-        rewrite lookup_branch_b_lookup_expr_branch in Hlookup_branch.
-        eapply first_payload_binder_branch_lookup_none; eassumption.
-      }
-      rewrite Hbinders_head in Hinfer.
-      assert (Hparams_head :
-        match_payload_params [] l0 l1 v_head = infer_ok []).
-      {
-        unfold match_payload_params, instantiate_enum_variant_field_tys.
-        rewrite Hfields_head. simpl. reflexivity.
-      }
-      rewrite Hparams_head in Hinfer. simpl in Hinfer.
-      destruct (infer_core_env_state_fuel_roots_shadow_safe fuel' env Ω n R1
-          (sctx_add_params [] Σ1) e_head)
-        as [[[[T_head Σ_head] R_out] roots_head] | err_head] eqn:Hhead;
+        eqn:Hlookup_branch; try discriminate.
+      destruct (match_payload_params binders_head l0 l1 v_head)
+        as [ps_head | err_params_head] eqn:Hparams_head; try discriminate.
+      destruct (params_names_nodup_b ps_head &&
+          ctx_lookup_params_none_b ps_head Σ1 &&
+          root_env_lookup_params_none_b ps_head R1) eqn:Hnodup_head;
+        try discriminate.
+      destruct (infer_core_env_state_fuel_roots_shadow_safe fuel' env Ω n
+          (root_env_add_params_roots_same ps_head roots_scrut R1)
+          (sctx_add_params ps_head Σ1) e_head)
+        as [[[[T_head Σ_head_payload] R_head_payload] roots_head] | err_head] eqn:Hhead;
+        try discriminate.
+      destruct (params_ok_sctx_b env ps_head Σ_head_payload &&
+          roots_exclude_params_b ps_head roots_head &&
+          root_env_excludes_params_b ps_head
+            (root_env_remove_match_params ps_head R_head_payload)) eqn:Hcleanup_head;
         try discriminate.
       remember
         ((fix infer_rest (T_head0 : Ty) (R_out0 : root_env)
@@ -1723,27 +1710,22 @@ Proof.
                     else infer_err (ErrTypeMismatch (ty_core T0) (ty_core T_head0))
                 | infer_err err => infer_err err
                 end
-            end) T_head R_out v_tail) as tail_result eqn:Htail.
+            end) T_head (root_env_remove_match_params ps_head R_head_payload) v_tail)
+        as tail_result eqn:Htail.
       destruct tail_result as [[[Σ_tail Ts_tail] roots_tail] | err_tail];
         try discriminate.
       symmetry in Htail.
-      assert (Hpayload_tail : first_payload_variant v_tail = None).
-      {
-        simpl in Hpayload.
-        destruct (enum_variant_fields v_head); try discriminate.
-        exact Hpayload.
-      }
       assert (Htail_typed :
         typed_match_tail_roots_shadow_safe env Ω n l0 l1 R1 roots_scrut Σ1 l v_tail
-          (ty_core T_head) R_out Σ_tail Ts_tail roots_tail).
+          (ty_core T_head) (root_env_remove_match_params ps_head R_head_payload)
+          Σ_tail Ts_tail roots_tail).
       {
-        clear Hinfer Hvariants Hunknown Hmissing Hdup Hunsupported Hpayload.
-        revert Σ_tail Ts_tail roots_tail Htail Hpayload_tail.
+        clear Hinfer Hvariants Hunknown Hmissing Hdup.
+        revert Σ_tail Ts_tail roots_tail Htail.
         induction v_tail as [|v rest IHtail];
-          intros Σ_tail Ts_tail roots_tail Htail0 Hpayload0; simpl in Htail0.
+          intros Σ_tail Ts_tail roots_tail Htail0; simpl in Htail0.
         - inversion Htail0; subst. constructor.
-        - simpl in Hpayload0.
-          destruct (enum_variant_fields v) eqn:Hfields; try discriminate.
+        -
           destruct (lookup_expr_branch_binders (enum_variant_name v) l)
             as [binders |] eqn:Hbinders0; try discriminate.
           destruct (lookup_branch_b (enum_variant_name v) l) as [e0 |]
@@ -1762,7 +1744,8 @@ Proof.
             eqn:Hcleanup_checks; try discriminate.
           destruct (ty_core_eqb (ty_core T0) (ty_core T_head)) eqn:Hcore0;
             try discriminate.
-          destruct (root_env_eqb (root_env_remove_match_params ps R0) R_out)
+          destruct (root_env_eqb (root_env_remove_match_params ps R0)
+              (root_env_remove_match_params ps_head R_head_payload))
             eqn:Hroot0; try discriminate.
           change (infer_if_bool true ?ok ?err) with ok in Htail0.
           remember
@@ -1819,93 +1802,110 @@ Proof.
                         else infer_err (ErrTypeMismatch (ty_core T1) (ty_core T_head0))
                     | infer_err err => infer_err err
                     end
-                end) T_head R_out rest) as tail0 eqn:Htail_rest.
+                end) T_head
+                  (root_env_remove_match_params ps_head R_head_payload)
+                  rest) as tail0 eqn:Htail_rest.
           destruct tail0 as [[[Σs Ts] rootss] | err_tail0]; try discriminate.
           inversion Htail0; subst.
           symmetry in Htail_rest.
           rewrite lookup_branch_b_lookup_expr_branch in Hlookup0.
-          assert (Hbinders_nil : binders = []).
-          {
-            pose proof (first_payload_binder_branch_lookup_none
-              l (enum_variant_name v) e0 Hbinders Hlookup0) as Hnone_lookup.
-            rewrite Hbinders0 in Hnone_lookup. inversion Hnone_lookup. reflexivity.
-          }
-          subst binders.
-          assert (Hps_nil : ps = []).
-          {
-            unfold match_payload_params, instantiate_enum_variant_field_tys in Hparams.
-            rewrite Hfields in Hparams. simpl in Hparams.
-            inversion Hparams. reflexivity.
-          }
-          subst ps.
-          simpl in Hparam_checks, Hcleanup_checks.
-	          eapply TERSMatchTail_Cons with
-            (R_payload := R1) (Rv_payload := R0) (Rv := R0)
-            (Σv_payload := Σ0) (Σv := Σ0)
-	            (Σs := Σs) (Ts := Ts) (rootss := rootss)
-	            (T := T0) (e := e0) (binders := []) (ps := [])
-	            (lts := l0) (args := l1) (roots_scrut := roots_scrut).
-		          + exact Hfields.
-		          + reflexivity.
-		          + exact Hbinders0.
-	          + unfold match_payload_params, instantiate_enum_variant_field_tys.
-            rewrite Hfields. simpl. reflexivity.
-          + reflexivity.
-          + reflexivity.
-          + reflexivity.
+          eapply TERSMatchTail_Cons with
+            (R_payload := root_env_add_params_roots_same ps roots_scrut R1)
+            (Rv_payload := R0) (Rv := root_env_remove_match_params ps R0)
+            (Σv_payload := Σ0) (Σv := sctx_remove_params ps Σ0)
+            (Σs := Σs) (Ts := Ts) (rootss := rootss)
+            (T := T0) (e := e0) (binders := binders) (ps := ps)
+            (lts := l0) (args := l1) (roots_scrut := roots_scrut).
+          + exact Hbinders0.
+          + exact Hparams.
+          + apply andb_prop in Hparam_checks as [Hnodup_rest Hrenv].
+            apply andb_prop in Hnodup_rest as [Hnodup _]. exact Hnodup.
+          + apply andb_prop in Hparam_checks as [Hnodup_rest Hrenv].
+            apply andb_prop in Hnodup_rest as [_ Hctx]. exact Hctx.
+          + apply andb_prop in Hparam_checks as [_ Hrenv]. exact Hrenv.
           + exact Hlookup0.
           + reflexivity.
           + eapply IH. exact Hinfer0.
+          + apply andb_prop in Hcleanup_checks as [Hok_rest Hrexcl].
+            apply andb_prop in Hok_rest as [Hok _]. exact Hok.
+          + apply andb_prop in Hcleanup_checks as [Hok_rest _].
+            apply andb_prop in Hok_rest as [_ Hexcl].
+            apply roots_exclude_params_b_sound_local. exact Hexcl.
           + reflexivity.
-          + constructor.
-          + reflexivity.
-          + constructor.
+          + apply andb_prop in Hcleanup_checks as [_ Hrexcl].
+            apply root_env_excludes_params_b_sound_local. exact Hrexcl.
           + reflexivity.
           + apply ty_core_eqb_true. exact Hcore0.
           + apply root_env_eqb_true_equiv. exact Hroot0.
-          + eapply IHtail.
-            * reflexivity.
-            * exact Hpayload0.
+          + eapply IHtail. reflexivity.
       }
-      destruct (ctx_merge_many (ctx_of_sctx Σ_head) (map ctx_of_sctx Σ_tail))
-        as [Γ_out |] eqn:Hmerge; try discriminate.
+      destruct (ctx_merge_many
+          (ctx_of_sctx (sctx_remove_params ps_head Σ_head_payload))
+          (map ctx_of_sctx Σ_tail)) as [Γ_out |] eqn:Hmerge; try discriminate.
+      assert (Hcalc :
+        infer_core_env_state_fuel_roots_shadow_safe (S fuel') env Ω n R Σ (EMatch e l) =
+        infer_ok
+          (MkTy (usage_max_tys_nonempty T_head Ts_tail) (ty_core T_head),
+           sctx_of_ctx Γ_out,
+           root_env_remove_match_params ps_head R_head_payload,
+           root_set_union roots_head (root_sets_union roots_tail))).
+      {
+        simpl in Hmissing.
+        simpl.
+        rewrite Hscrut, Hscrut_core, Hlookup, Hlts, Hargslen, Hbounds,
+          Hdup, Hvariants.
+        simpl.
+        rewrite Hunknown, Hmissing.
+        rewrite Hbinders_head, Hlookup_branch, Hparams_head, Hnodup_head,
+          Hhead.
+        simpl.
+        destruct (params_ok_sctx_b env ps_head Σ_head_payload &&
+            roots_exclude_params_b ps_head roots_head &&
+            root_env_excludes_params_b ps_head
+              (root_env_remove_match_params ps_head R_head_payload)) eqn:Hcleanup;
+          [| rewrite Hcleanup_head in Hcleanup; discriminate].
+        simpl.
+        rewrite Htail.
+        simpl.
+        rewrite Hmerge.
+        reflexivity.
+      }
       inversion Hinfer; subst.
       rewrite lookup_branch_b_lookup_expr_branch in Hlookup_branch.
-      change (typed_env_roots_shadow_safe env Ω n R Σ (EMatch e l)
-        (MkTy (usage_max_tys_nonempty T_head Ts_tail) (ty_core T_head))
-        (sctx_of_ctx Γ_out) R'
-        (root_set_union roots_head (root_sets_union roots_tail))).
-	      eapply TERS_Match with
-        (R1 := R1) (R_payload := R1) (R_head_payload := R')
-        (R_out := R') (Σ1 := Σ1) (Σ_head_payload := Σ_head)
-        (Σ_head := Σ_head) (Σ_tail := Σ_tail)
+      eapply TERS_Match with
+        (R1 := R1)
+        (R_payload := root_env_add_params_roots_same ps_head roots_scrut R1)
+        (R_head_payload := R_head_payload)
+        (R_out := root_env_remove_match_params ps_head R_head_payload)
+        (Σ1 := Σ1) (Σ_head_payload := Σ_head_payload)
+        (Σ_head := sctx_remove_params ps_head Σ_head_payload)
+        (Σ_tail := Σ_tail)
         (Γ_out := Γ_out) (edef := edef) (v_head := v_head)
         (v_tail := v_tail) (e_head := e_head) (T_scrut := T_scrut)
         (T_head := T_head) (Ts_tail := Ts_tail)
         (roots_scrut := roots_scrut) (roots_head := roots_head)
-        (roots_tail := roots_tail) (binders_head := []) (ps_head := []);
+        (roots_tail := roots_tail)
+        (binders_head := binders_head) (ps_head := ps_head);
         [ eapply IH; exact Hscrut
         | exact Hscrut_core
         | exact Hlookup
         | apply negb_false_iff in Hlts; apply Nat.eqb_eq in Hlts; exact Hlts
         | apply negb_false_iff in Hargslen; apply Nat.eqb_eq in Hargslen; exact Hargslen
-	        | exact Hbounds
-	        | rewrite Hvariants; exact Hunknown
-	        | exact Hvariants
-		        | exact Hfields_head
-		        | reflexivity
-		        | exact Hbinders_head
-	        | exact Hparams_head
-        | reflexivity
-        | reflexivity
-        | reflexivity
+        | exact Hbounds
+        | rewrite Hvariants; exact Hunknown
+        | exact Hvariants
+        | exact Hbinders_head
+        | exact Hparams_head
+        | apply andb_prop in Hnodup_head as [Hnd_rest Hrenv]; apply andb_prop in Hnd_rest as [Hnd _]; exact Hnd
+        | apply andb_prop in Hnodup_head as [Hnd_rest Hrenv]; apply andb_prop in Hnd_rest as [_ Hctx]; exact Hctx
+        | apply andb_prop in Hnodup_head as [_ Hrenv]; exact Hrenv
         | exact Hlookup_branch
         | reflexivity
         | eapply IH; exact Hhead
+        | apply andb_prop in Hcleanup_head as [Hok_rest Hrexcl]; apply andb_prop in Hok_rest as [Hok _]; exact Hok
+        | apply andb_prop in Hcleanup_head as [Hok_rest _]; apply andb_prop in Hok_rest as [_ Hexcl]; apply roots_exclude_params_b_sound_local; exact Hexcl
         | reflexivity
-        | constructor
-        | reflexivity
-        | constructor
+        | apply andb_prop in Hcleanup_head as [_ Hrexcl]; apply root_env_excludes_params_b_sound_local; exact Hrexcl
         | reflexivity
         | exact Htail_typed
         | exact Hmerge ];
